Unproven file_set_attr. Maybe exclude updating the length attribute?  Now the spec isn't quite right, and probably unprovable without some extra promises from the caller. Other option is to add an extra precondition that states new length is equal to old length, which is true for our one use case.

src/FS.v
@@ -171,6 +171,35 @@ Qed.
 
 Hint Extern 1 ({{_}} progseq (file_get_attr _ _ _) _) => apply file_getattr_ok : prog.
 
+Definition file_set_attr T fsxp inum attr mscs rx : prog T :=
+  mscs <- LOG.begin (FSXPLog fsxp) mscs;
+  mscs <- DIRTREE.setattr fsxp inum attr mscs;
+  let^ (mscs, ok) <- LOG.commit (FSXPLog fsxp) mscs;
+  rx ^(mscs, ok).
+
+Theorem file_setattr_ok : forall fsxp inum newattr mscs,
+  {< m pathname Fm Ftop tree bytes attr,
+  PRE    LOG.rep (FSXPLog fsxp) (sb_rep fsxp) (NoTransaction m) mscs *
+         [[ (Fm * DIRTREE.rep fsxp Ftop tree)%pred (list2mem m) ]] *
+         [[ DIRTREE.find_subtree pathname tree = Some (DIRTREE.TreeFile inum bytes attr) ]]
+  POST RET:^(mscs, ok)
+         [[ ok = false ]] * LOG.rep fsxp.(FSXPLog) (sb_rep fsxp) (NoTransaction m) mscs \/
+         [[ ok = true ]] *
+         exists m' tree',
+         LOG.rep fsxp.(FSXPLog) (sb_rep fsxp) (NoTransaction m') mscs *   
+         [[ (Fm * DIRTREE.rep fsxp Ftop tree')%pred (list2mem m') ]] *
+         [[ tree' = DIRTREE.update_subtree pathname (DIRTREE.TreeFile inum bytes newattr) tree ]]
+  CRASH  LOG.would_recover_either_pred (FSXPLog fsxp)  (sb_rep fsxp) m (
+           exists tree',
+         (Fm * DIRTREE.rep fsxp Ftop tree') *
+         [[ tree' = DIRTREE.update_subtree pathname (DIRTREE.TreeFile inum bytes newattr) tree ]])
+  >} file_set_attr fsxp inum newattr mscs.
+Proof.
+  (* XXX prove *)
+Admitted.
+
+Hint Extern 1 ({{_}} progseq (file_set_attr _ _ _ _) _) => apply file_setattr_ok : prog.
+
 Ltac recover_ro_ok := intros;
   repeat match goal with 
   | [ |- forall_helper _ ] => idtac "forall"; unfold forall_helper; intros; eexists; intros
@@ -191,7 +220,6 @@ Ltac recover_ro_ok := intros;
   | [ |- pimpl (LOG.would_recover_either_pred _ _ _ _ ) _ ] => idtac "would_rec";
        rewrite LOG.would_recover_either_pred_diskIs_rev by auto; cancel
   end.
-
 
 Theorem file_getattr_recover_ok : forall fsxp inum mscs,
   {<< m pathname Fm Ftop tree bytes attr,
